lean/Coercions/Classifiers/FCdot/Consistency.lean
@@ -59,6 +59,11 @@ theorem EntryTyped.bnd_of_bndsOnly {ρ : Option (BVar s .var)} {TelM : Telescope
   | kindC hh _ _ =>
       cases hh with
       | kindC hAt => obtain ⟨_, hP⟩ := hb _ _ hAt; exact absurd hP (by simp)
+  | kindCle hh _ _ _ =>
+      cases hh with
+      | leC hAt => obtain ⟨_, hP⟩ := hb _ _ hAt; exact absurd hP (by simp)
+      | eqC hAt => obtain ⟨_, hP⟩ := hb _ _ hAt; exact absurd hP (by simp)
+      | eqSymC hAt => obtain ⟨_, hP⟩ := hb _ _ hAt; exact absurd hP (by simp)
   | eqC hAt => obtain ⟨_, hP⟩ := hb _ _ hAt; exact absurd hP (by simp)
   | eqSymC hAt => obtain ⟨_, hP⟩ := hb _ _ hAt; exact absurd hP (by simp)
 
